Using refinement in dynamic array.

HOL/SepLogic/DynamicArray.thy
@@ -1,77 +1,185 @@
 theory DynamicArray
-imports SepAuto "../DataStrs/Arrays_Ex"
+imports Arrays_Impl
 begin
 
-datatype 'a dynamic_array = Dyn_Array (alen: nat) (amax: nat) (aref: "'a array")
+datatype 'a dynamic_array = Dyn_Array (alen: nat) (aref: "'a array")
 setup {* add_rewrite_rule_back @{thm dynamic_array.collapse} *}
 setup {* add_rewrite_rule @{thm dynamic_array.case} *}
 setup {* fold add_rewrite_rule @{thms dynamic_array.sel} *}
 
-fun dyn_array :: "'a::heap list \<Rightarrow> 'a dynamic_array \<Rightarrow> assn" where
-  "dyn_array xs (Dyn_Array al am a) =
-     (\<exists>\<^sub>Axs'. a \<mapsto>\<^sub>a xs' * \<up>(xs = take al xs') * \<up>(al \<le> length xs') * \<up>(am = length xs'))"
-setup {* add_rewrite_ent_rule @{thm dyn_array.simps} *}
+section {* Raw assertion *}
+
+fun dyn_array_raw :: "'a::heap list \<times> nat \<Rightarrow> 'a dynamic_array \<Rightarrow> assn" where
+  "dyn_array_raw (xs, n) (Dyn_Array m a) = (a \<mapsto>\<^sub>a xs * \<up>(m = n))"
+setup {* add_rewrite_ent_rule @{thm dyn_array_raw.simps} *}
 
 definition dyn_array_new :: "'a::heap dynamic_array Heap" where [sep_proc]:
   "dyn_array_new = do {
      p \<leftarrow> Array.new 5 undefined;
-     return (Dyn_Array 0 5 p)
+     return (Dyn_Array 0 p)
    }"
 
-lemma dyn_array_new_rule [hoare_triple]:
-  "<emp> dyn_array_new <dyn_array []>" by auto2
+lemma dyn_array_new_rule' [hoare_triple]:
+  "<emp>
+   dyn_array_new
+   <dyn_array_raw (replicate 5 undefined, 0)>" by auto2
 
-fun array_copy :: "'a::heap array \<Rightarrow> 'a array \<Rightarrow> nat \<Rightarrow> unit Heap" where
-  "array_copy a b 0 = (return ())"
-| "array_copy a b (Suc n) = do {
-      array_copy a b n;
-      x \<leftarrow> Array.nth a n;
-      Array.upd n x b;
-      return () }"
-declare array_copy.simps [sep_proc]
-
-lemma array_copy_rule [hoare_triple]:
-  "n \<le> length as \<Longrightarrow> n \<le> length bs \<Longrightarrow>
-   <a \<mapsto>\<^sub>a as * b \<mapsto>\<^sub>a bs>
-    array_copy a b n
-   <\<lambda>_. a \<mapsto>\<^sub>a as * b \<mapsto>\<^sub>a Arrays_Ex.array_copy as bs n>"
-@proof @induct n @qed
-
-definition ensure_length :: "'a::heap dynamic_array \<Rightarrow> 'a dynamic_array Heap" where [sep_proc]:
-  "ensure_length d = (case d of Dyn_Array al am ar \<Rightarrow>
-    if al < am then return d
-    else do {
+definition double_length :: "'a::heap dynamic_array \<Rightarrow> 'a dynamic_array Heap" where [sep_proc]:
+  "double_length d = (case d of Dyn_Array al ar \<Rightarrow> do {
+      am \<leftarrow> Array.len ar;
       p \<leftarrow> Array.new (2 * am + 1) undefined;
       array_copy ar p am;
-      return (Dyn_Array am (2 * am + 1) p)
+      return (Dyn_Array am p)
     })"
 
-lemma ensure_length_rule [hoare_triple]:
-  "<dyn_array xs p>
-   ensure_length p
-   <\<lambda>r. dyn_array xs r * \<up>(alen r < amax r)>\<^sub>t" by auto2
+fun double_length_fun :: "'a::heap list \<times> nat \<Rightarrow> 'a list \<times> nat" where
+  "double_length_fun (xs, n) =
+    (Arrays_Ex.array_copy xs (replicate (2 * n + 1) undefined) n, n)"
+setup {* add_rewrite_rule @{thm double_length_fun.simps} *}
 
-definition push_array :: "'a \<Rightarrow> 'a::heap dynamic_array \<Rightarrow> 'a dynamic_array Heap" where [sep_proc]:
-  "push_array x d = do {
-    p \<leftarrow> ensure_length d;
-    Array.upd (alen d) x (aref p);
-    return (Dyn_Array (alen p + 1) (amax p) (aref p))
+lemma double_length_rule' [hoare_triple]:
+  "length xs = n \<Longrightarrow>
+   <dyn_array_raw (xs, n) p>
+   double_length p
+   <dyn_array_raw (double_length_fun (xs, n))>\<^sub>t" by auto2
+
+definition push_array_basic :: "'a \<Rightarrow> 'a::heap dynamic_array \<Rightarrow> 'a dynamic_array Heap" where [sep_proc]:
+  "push_array_basic x p = do {
+    Array.upd (alen p) x (aref p);
+    return (Dyn_Array (alen p + 1) (aref p))
    }"
 
-lemma push_array_rule [hoare_triple]:
-  "<dyn_array xs p>
+fun push_array_basic_fun :: "'a \<Rightarrow> 'a::heap list \<times> nat \<Rightarrow> 'a list \<times> nat" where
+  "push_array_basic_fun x (xs, n) = (list_update xs n x, n + 1)"
+setup {* add_rewrite_rule @{thm push_array_basic_fun.simps} *}
+
+lemma push_array_basic_rule' [hoare_triple]:
+  "n < length xs \<Longrightarrow>
+   <dyn_array_raw (xs, n) p>
+   push_array_basic x p
+   <dyn_array_raw (push_array_basic_fun x (xs, n))>" by auto2
+
+definition array_length :: "'a dynamic_array \<Rightarrow> nat Heap" where [sep_proc]:
+  "array_length d = return (alen d)"
+
+lemma array_length_heap_preserving [heap_presv]:
+  "heap_preserving (array_length d)" by auto2
+
+lemma array_length_rule' [hoare_triple]:
+  "<dyn_array_raw (xs, n) p>
+   array_length p
+   <\<lambda>r. dyn_array_raw (xs, n) p * \<up>(r = n)>" by auto2
+
+definition array_max :: "'a::heap dynamic_array \<Rightarrow> nat Heap" where [sep_proc]:
+  "array_max d = Array.len (aref d)"
+
+lemma array_max_rule' [hoare_triple]:
+  "<dyn_array_raw (xs, n) p>
+   array_max p
+   <\<lambda>r. dyn_array_raw (xs, n) p * \<up>(r = length xs)>" by auto2
+
+definition array_nth :: "'a::heap dynamic_array \<Rightarrow> nat \<Rightarrow> 'a Heap" where [sep_proc]:
+  "array_nth d i = Array.nth (aref d) i"
+
+lemma array_nth_heap_preserving [heap_presv]:
+  "heap_preserving (array_nth d i)" by auto2
+
+lemma array_nth_rule' [hoare_triple]:
+  "i < n \<Longrightarrow> n \<le> length xs \<Longrightarrow>
+   <dyn_array_raw (xs, n) p>
+   array_nth p i
+   <\<lambda>r. dyn_array_raw (xs, n) p * \<up>(r = xs ! i)>" by auto2
+
+definition array_upd :: "nat \<Rightarrow> 'a \<Rightarrow> 'a::heap dynamic_array \<Rightarrow> unit Heap" where [sep_proc]:
+  "array_upd i x d = do { Array.upd i x (aref d); return () }"
+
+lemma array_upd_rule' [hoare_triple]:
+  "i < n \<Longrightarrow> n \<le> length xs \<Longrightarrow>
+   <dyn_array_raw (xs, n) p>
+   array_upd i x p
+   <\<lambda>_. dyn_array_raw (list_update xs i x, n) p>" by auto2
+
+definition push_array :: "'a \<Rightarrow> 'a::heap dynamic_array \<Rightarrow> 'a dynamic_array Heap" where [sep_proc]:
+  "push_array x p = do {
+    m \<leftarrow> array_max p;
+    l \<leftarrow> array_length p;
+    if l < m then push_array_basic x p
+    else do {
+      u \<leftarrow> double_length p;
+      push_array_basic x u
+    }
+  }"
+
+fun push_array_fun :: "'a \<Rightarrow> 'a::heap list \<times> nat \<Rightarrow> 'a list \<times> nat" where
+  "push_array_fun x (xs, n) = (
+     if n < length xs then push_array_basic_fun x (xs, n)
+     else push_array_basic_fun x (double_length_fun (xs, n)))"
+setup {* add_rewrite_rule @{thm push_array_fun.simps} *}
+
+lemma push_array_rule' [hoare_triple]:
+  "n \<le> length xs \<Longrightarrow>
+   <dyn_array_raw (xs, n) p>
    push_array x p
-   <dyn_array (xs @ [x])>\<^sub>t"
-@proof @have "length (xs @ [x]) = length xs + 1" @qed
+   <dyn_array_raw (push_array_fun x (xs, n))>\<^sub>t" by auto2
 
 definition pop_array :: "'a::heap dynamic_array \<Rightarrow> ('a \<times> 'a dynamic_array) Heap" where [sep_proc]:
   "pop_array d = do {
     x \<leftarrow> Array.nth (aref d) (alen d - 1);
-    return (x, Dyn_Array (alen d - 1) (amax d) (aref d))
+    return (x, Dyn_Array (alen d - 1) (aref d))
    }"
 
-lemma pop_array_heap_preserving [heap_presv]:
-  "heap_preserving (pop_array d)" by auto2
+lemma pop_array_rule' [hoare_triple]:
+  "n > 0 \<Longrightarrow> n \<le> length xs \<Longrightarrow>
+   <dyn_array_raw (xs, n) p>
+   pop_array p
+   <\<lambda>(x, r). dyn_array_raw (xs, n - 1) r * \<up>(x = xs ! (n - 1))>" by auto2
+
+setup {* del_prfstep_thm @{thm dyn_array_raw.simps} *}
+setup {* del_prfstep_thm @{thm dynamic_array.collapse} *}
+
+section {* Abstract assertion *}
+
+fun abs_array :: "'a::heap list \<times> nat \<Rightarrow> 'a list" where
+  "abs_array (xs, n) = take n xs"
+setup {* add_rewrite_rule @{thm abs_array.simps} *}
+
+lemma double_length_abs [rewrite]:
+  "length xs = n \<Longrightarrow> abs_array (double_length_fun (xs, n)) = abs_array (xs, n)" by auto2
+
+lemma push_array_basic_abs [rewrite]:
+  "n < length xs \<Longrightarrow> abs_array (push_array_basic_fun x (xs, n)) = abs_array (xs, n) @ [x]"
+@proof @have "length (take n xs @ [x]) = n + 1" @qed
+
+lemma push_array_fun_abs [rewrite]:
+  "n \<le> length xs \<Longrightarrow> abs_array (push_array_fun x (xs, n)) = abs_array (xs, n) @ [x]" by auto2
+
+definition dyn_array :: "'a::heap list \<Rightarrow> 'a dynamic_array \<Rightarrow> assn" where [rewrite_ent]:
+  "dyn_array xs a = (\<exists>\<^sub>Ap. dyn_array_raw p a * \<up>(xs = abs_array p) * \<up>(snd p \<le> length (fst p)))"
+
+lemma dyn_array_new_rule [hoare_triple]:
+  "<emp> dyn_array_new <dyn_array []>" by auto2
+
+lemma array_length_rule [hoare_triple]:
+  "<dyn_array xs p>
+   array_length p
+   <\<lambda>r. dyn_array xs p * \<up>(r = length xs)>" by auto2
+
+lemma array_nth_rule [hoare_triple]:
+  "i < length xs \<Longrightarrow>
+   <dyn_array xs p>
+    array_nth p i
+   <\<lambda>r. dyn_array xs p * \<up>(r = xs ! i)>" by auto2
+
+lemma array_upd_rule [hoare_triple]:
+  "i < length xs \<Longrightarrow>
+   <dyn_array xs p>
+    array_upd i x p
+   <\<lambda>_. dyn_array (list_update xs i x) p>" by auto2
+
+lemma push_array_rule [hoare_triple]:
+  "<dyn_array xs p>
+    push_array x p
+   <dyn_array (xs @ [x])>\<^sub>t" by auto2
 
 lemma pop_array_rule [hoare_triple]:
   "xs \<noteq> [] \<Longrightarrow>
@@ -80,40 +188,7 @@ lemma pop_array_rule [hoare_triple]:
    <\<lambda>(x, r). dyn_array (butlast xs) r * \<up>(x = last xs)>"
 @proof @have "last xs = xs ! (length xs - 1)" @qed
 
-definition array_upd :: "nat \<Rightarrow> 'a \<Rightarrow> 'a::heap dynamic_array \<Rightarrow> unit Heap" where [sep_proc]:
-  "array_upd i x d = do { Array.upd i x (aref d); return () }"
-
-lemma array_upd_rule [hoare_triple]:
-  "i < length xs \<Longrightarrow>
-   <dyn_array xs p>
-   array_upd i x p
-   <\<lambda>_. dyn_array (list_update xs i x) p>" by auto2
-
-definition array_nth :: "'a::heap dynamic_array \<Rightarrow> nat \<Rightarrow> 'a Heap" where [sep_proc]:
-  "array_nth d i = Array.nth (aref d) i"
-
-lemma array_nth_heap_preserving [heap_presv]:
-  "heap_preserving (array_nth d i)" by auto2
-
-lemma array_nth_rule [hoare_triple]:
-  "i < length xs \<Longrightarrow>
-   <dyn_array xs p>
-   array_nth p i
-   <\<lambda>r. dyn_array xs p * \<up>(r = xs ! i)>" by auto2
-
-definition array_length :: "'a dynamic_array \<Rightarrow> nat Heap" where [sep_proc]:
-  "array_length d = return (alen d)"
-
-lemma array_length_heap_preserving [heap_presv]:
-  "heap_preserving (array_length d)" by auto2
-
-lemma array_length_rule [hoare_triple]:
-  "<dyn_array xs p>
-   array_length p
-   <\<lambda>r. dyn_array xs p * \<up>(r = length xs)>" by auto2
-
-setup {* del_prfstep_thm @{thm dynamic_array.collapse} *}
-setup {* fold del_prfstep_thm @{thms dyn_array.simps} *}
+section {* Derived operations *}
 
 definition array_swap :: "'a::heap dynamic_array \<Rightarrow> nat \<Rightarrow> nat \<Rightarrow> unit Heap" where [sep_proc]:
   "array_swap d i j = do {
@@ -129,5 +204,7 @@ lemma array_swap_rule [hoare_triple]:
    <dyn_array xs p>
    array_swap p i j
    <\<lambda>_. dyn_array (list_swap xs i j) p>" by auto2
+
+setup {* del_prfstep_thm @{thm dyn_array_def} *}
 
 end
