HOL/SepLogic/Arrays_Impl.thy
@@ -1,0 +1,21 @@
+theory Arrays_Impl
+  imports SepAuto "../DataStrs/Arrays_Ex"
+begin
+
+fun array_copy :: "'a::heap array \<Rightarrow> 'a array \<Rightarrow> nat \<Rightarrow> unit Heap" where
+  "array_copy a b 0 = (return ())"
+| "array_copy a b (Suc n) = do {
+      array_copy a b n;
+      x \<leftarrow> Array.nth a n;
+      Array.upd n x b;
+      return () }"
+declare array_copy.simps [sep_proc]
+
+lemma array_copy_rule [hoare_triple]:
+  "n \<le> length as \<Longrightarrow> n \<le> length bs \<Longrightarrow>
+   <a \<mapsto>\<^sub>a as * b \<mapsto>\<^sub>a bs>
+    array_copy a b n
+   <\<lambda>_. a \<mapsto>\<^sub>a as * b \<mapsto>\<^sub>a Arrays_Ex.array_copy as bs n>"
+@proof @induct n @qed
+
+end
